Lp2lc/Active/STLC/__Infer.lean
@@ -30,7 +30,7 @@ def infer [env: @BuildEnv F] (self : Trm F) : RecOpt (Typ F)
     match self with
     | .val (.lit _) => .yield (some .primitive)
     | .val (.lam body tIn) =>
-      let index := env.trm2typCtx.getUID ⟨self, tIn⟩
+      let index := env.trm2typCtx.getUId ⟨self, tIn⟩
       ((body index).infer fuel).map (λ out => out.map (λ tOut => .fn tIn tOut))
     | .apply fnTerm arg =>
       match fnTerm.infer fuel, arg.infer fuel with
@@ -62,11 +62,11 @@ theorem termInferMonotone [env : @BuildEnv F]
           | lit repr => simpa [AST.infer] using hInfer
           | lam body tIn =>
             cases hBody :
-                (body (env.trm2typCtx.getUID ⟨.val (.lam body tIn), tIn⟩)).infer fuel with
+                (body (env.trm2typCtx.getUId ⟨.val (.lam body tIn), tIn⟩)).infer fuel with
             | outOfFuel => simp [AST.infer, hBody, Outcome.map] at hInfer
             | yield bodyResult =>
               have hBodyTop := ih fuel (Nat.lt_succ_self fuel)
-                (body (env.trm2typCtx.getUID ⟨.val (.lam body tIn), tIn⟩))
+                (body (env.trm2typCtx.getUId ⟨.val (.lam body tIn), tIn⟩))
                 toFuel bodyResult hFuelTail hBody
               simpa [AST.infer, Outcome.map, hBody, hBodyTop] using hInfer
         | apply fnTerm arg =>
@@ -107,7 +107,7 @@ There are few intricacies:
   - `t.infer` should work even in this case
 - the subtyping symbol `<=` is only applicable for AST with identical carrier, so `infer` is allowed to shift carrier, but `eval` is not
 
-To avoid UID being abused to fake construction from any Fixpoint, the simple conjecture should be:
+To avoid UId being abused to fake construction from any Fixpoint, the simple conjecture should be:
 
 []
 
